Add files via upload

Verif_swap.v
@@ -24,7 +24,6 @@ Qed.
 Lemma prove_emp: emp |-- emp.
 Proof. auto. Qed. 
 
-
 (*swap specification*)
 Definition swap_spec : ident * funspec :=
   DECLARE _swap
@@ -40,6 +39,21 @@ Definition swap_spec : ident * funspec :=
     (*SEP(emp)*)
     SEP (data_at sh1 tint (Vint (Int.repr b)) x; data_at sh2 tint (Vint (Int.repr a)) y).
 
+(*swap-skip specification - point to the same variable*)
+Definition swapskip_spec : ident * funspec :=
+  DECLARE _swapskip
+   WITH x: val, y: val, sh1 : share, sh2 : share, a : Z, b : Z
+   PRE [ tptr tint, tptr tint ]
+    PROP  (writable_share sh1; writable_share sh2)
+    (*LOCAL (temp _x x; temp _y y)*)
+    PARAMS (x; y)
+    (*SEP(emp)*)
+    SEP (data_at sh1 tint (Vint (Int.repr a)) x; data_at sh2 tint (Vint (Int.repr b)) y)
+   POST [ tvoid ]
+    PROP () RETURN ()
+    (*SEP(emp)*)
+    SEP (data_at sh1 tint (Vint (Int.repr a)) x; data_at sh2 tint (Vint (Int.repr b)) y).
+
 (*varspec: global variables
   funspec: set of functions (Gprog)
   function: function should be a member of funspec
@@ -51,49 +65,139 @@ Definition swap_spec : ident * funspec :=
  P and Q: PROP, LOCAL and SEP; 
  Read: Add stuff to LOCAL*)
 
-Definition Gprog := [swap_spec].
+Definition Gprog := [swapskip_spec; swap_spec].
 
+Check f_swap.
 
-Lemma body_swap: semax_body Vprog Gprog f_swap swap_spec.
+Compute (check_norm_stmt (fn_body f_swapskip)).
+Compute (fn_body f_swapskip).
+Compute (fn_callconv f_swapskip).
+Locate fn_body.
+Print fn_body.
+Check f_swapskip.
+Print fn_body.
+Check check_norm_stmt.
+
+(*no ltacs used*)
+Lemma body_swapskip: semax_body Vprog Gprog f_swapskip swapskip_spec.
 Proof.
-  start_function.
-  eapply semax_seq with (Q := PROP ( )
-  LOCAL (temp _a2 (Vint (Int.repr a));temp _x x; temp _y y)
-  SEP (data_at sh1 tint (Vint (Int.repr a)) x;
-  data_at sh2 tint (Vint (Int.repr b)) y)). 
-  Print load_tac.
-  (*unable to apply load_tac and semax_SC_set*) 
-  (*eapply semax_SC_set.
-  Print semax_seq.
+  start_function. unfold POSTCONDITION. unfold abbreviate.
+  unfold stackframe_of. simpl map. rewrite fold_right_nil.
+  rewrite sepcon_emp.
+  eapply semax_post. 5:{ eapply semax_skip. }
+  apply derives_ENTAIL. eapply drop_LOCAL'' with (n := O). eapply drop_LOCAL'' with (n := O). simpl. 
+  intros. entailer!.
+  apply derives_ENTAIL.
+  simpl. intros. entailer!.
+  simpl. intros. entailer!. simpl. intros. entailer!.
+  Qed.
 
+  Require Import VST.floyd.local2ptree_denote.
+  Require Import VST.floyd.local2ptree_eval.
+  Import compcert.lib.Maps.
+  (*very limited ltacs*)
+  Lemma body_swaplimltac: semax_body Vprog Gprog f_swap swap_spec.
+  Proof.
+    start_function. unfold POSTCONDITION. unfold abbreviate.
+    eapply semax_seq'.
+    (*first read*)
+   apply semax_later_trivial. 
+   Print Ltac load_tac. Locate load_tac.
+   match goal with
+   | |- semax ?Delta (|> (PROPx ?P (LOCALx ?Q (SEPx ?R)))) (Sset _ ?e) _ =>
+     let T1 := fresh "T1" in evar (T1: PTree.t val);
+     let T2 := fresh "T2" in evar (T2: PTree.t (type * val));
+     let G := fresh "GV" in evar (G: option globals);
+     let LOCAL2PTREE := fresh "LOCAL2PTREE" in
+     assert (local2ptree Q = (T1, T2, nil, G)) as LOCAL2PTREE;
+     [subst T1 T2 G; prove_local2ptree |];
+     first [ load_tac_with_hint LOCAL2PTREE | load_tac_no_hint LOCAL2PTREE | SEP_type_contradict LOCAL2PTREE Delta e R | hint_msg LOCAL2PTREE Delta e];
+     clear T1 T2 G LOCAL2PTREE
+   end.
+   unfold MORE_COMMANDS. unfold abbreviate. 
+   (*semax_seq -> read again*)
+   eapply semax_seq'. simpl. apply semax_later_trivial. 
+   match goal with
+   | |- semax ?Delta (|> (PROPx ?P (LOCALx ?Q (SEPx ?R)))) (Sset _ ?e) _ =>
+     let T1 := fresh "T1" in evar (T1: PTree.t val);
+     let T2 := fresh "T2" in evar (T2: PTree.t (type * val));
+     let G := fresh "GV" in evar (G: option globals);
+     let LOCAL2PTREE := fresh "LOCAL2PTREE" in
+     assert (local2ptree Q = (T1, T2, nil, G)) as LOCAL2PTREE;
+     [subst T1 T2 G; prove_local2ptree |];
+     first [ load_tac_with_hint LOCAL2PTREE | load_tac_no_hint LOCAL2PTREE | SEP_type_contradict LOCAL2PTREE Delta e R | hint_msg LOCAL2PTREE Delta e];
+     clear T1 T2 G LOCAL2PTREE
+   end.
+   (*semax seq -> write*)
+   eapply semax_seq'. simpl. apply semax_later_trivial.
+   (*store tac*) 
+   match goal with
+   | |- semax ?Delta (|> (PROPx ?P (LOCALx ?Q (SEPx ?R)))) (Sassign ?e1 ?e2) _ =>
+     check_expression_by_value e1;
+     let T1 := fresh "T1" in evar (T1: PTree.t val);
+     let T2 := fresh "T2" in evar (T2: PTree.t (type * val));
+     let G := fresh "GV" in evar (G: option globals);
+     let LOCAL2PTREE := fresh "LOCAL2PTREE" in
+     assert (local2ptree Q = (T1, T2, nil, G)) as LOCAL2PTREE;
+     [subst T1 T2 G; prove_local2ptree |];
+     first [ store_tac_with_hint LOCAL2PTREE | store_tac_no_hint LOCAL2PTREE | SEP_type_contradict LOCAL2PTREE Delta e1 R | hint_msg LOCAL2PTREE Delta e1];
+     clear T1 T2 LOCAL2PTREE
+   end.
+   (*skip and sequence and write*)
+   apply semax_seq_skip.  eapply semax_seq'. simpl.
+   apply semax_later_trivial; 
+   (*store tac*)
+   match goal with
+   | |- semax ?Delta (|> (PROPx ?P (LOCALx ?Q (SEPx ?R)))) (Sassign ?e1 ?e2) _ =>
+     check_expression_by_value e1;
+     let T1 := fresh "T1" in evar (T1: PTree.t val);
+     let T2 := fresh "T2" in evar (T2: PTree.t (type * val));
+     let G := fresh "GV" in evar (G: option globals);
+     let LOCAL2PTREE := fresh "LOCAL2PTREE" in
+     assert (local2ptree Q = (T1, T2, nil, G)) as LOCAL2PTREE;
+     [subst T1 T2 G; prove_local2ptree |];
+     first [ store_tac_with_hint LOCAL2PTREE | store_tac_no_hint LOCAL2PTREE | SEP_type_contradict LOCAL2PTREE Delta e1 R | hint_msg LOCAL2PTREE Delta e1];
+     clear T1 T2 LOCAL2PTREE
+   end.
+   (*skip part*)
+   unfold stackframe_of. simpl map. rewrite fold_right_nil.
+  rewrite sepcon_emp. simpl.
+  eapply semax_post. 5:{ eapply semax_skip. }
+  apply derives_ENTAIL. eapply drop_LOCAL'' with (n := O). eapply drop_LOCAL'' with (n := O).
+  eapply drop_LOCAL'' with (n := O). eapply drop_LOCAL'' with (n := O). simpl. 
+  intros. entailer!.
+  apply derives_ENTAIL.
+  simpl. intros. entailer!.
+  simpl. intros. entailer!. simpl. intros. entailer!.
+  Qed.
 
-
-  unfold POSTCONDITION. unfold abbreviate.
-
-  try unfold stackframe_of. simpl fn_vars. simpl map.
-      simple eapply canonicalize_stackframe.
-  unfold stackframe_of. simpl map. simpl. s
-  
-  Search fold_right nil.
-  rewrite fold_right_nil. Print emp_sepcon. Search emp. 
-  Print frame_ret_assert. Search normal_ret_assert emp.
-  Print emp_sepcon. rewrite <- emp_sepcon.
-  
-  rewrite frame_ret_assert_emp.
-
-  forward. unfold stackframe_of. simpl. simpl.
-  apply sepcon_derives.
-
-  eapply semax_skip.
-
-  
-  
-  unfold abbreviate in POSTCONDITION.
-  Check normal_ret_assert. unfold normal_ret_assert in POSTCONDITION.
-  Check RA_normal. Check RA_break.
-  Check POSTCONDITION.(RA_normal). *)
-
-Admitted.
+  (*limited ltacs*)
+  Lemma body_swapnoltac: semax_body Vprog Gprog f_swap swap_spec.
+   Proof.
+    Locate start_function.
+     start_function. unfold POSTCONDITION. unfold abbreviate.
+     eapply semax_seq'.
+     (*first read*)
+    apply semax_later_trivial. load_tac.
+    unfold MORE_COMMANDS. unfold abbreviate. 
+    (*semax_seq -> read again*)
+    eapply semax_seq'. simpl. apply semax_later_trivial; load_tac.
+    (*semax seq -> write*)
+    eapply semax_seq'. simpl. apply semax_later_trivial; store_tac.
+    (*read again*)
+    apply semax_seq_skip.  eapply semax_seq'. simpl.
+    apply semax_later_trivial; store_tac. 
+    (*skip part*)
+    unfold stackframe_of. simpl map. rewrite fold_right_nil.
+   rewrite sepcon_emp. simpl.
+   eapply semax_post. 5:{ eapply semax_skip. }
+   apply derives_ENTAIL. eapply drop_LOCAL'' with (n := O). eapply drop_LOCAL'' with (n := O).
+   eapply drop_LOCAL'' with (n := O). eapply drop_LOCAL'' with (n := O). simpl. 
+   intros. entailer!.
+   apply derives_ENTAIL.
+   simpl. intros. entailer!.
+   simpl. intros. entailer!. simpl. intros. entailer!.
+   Qed.
 
 (*explicit - forward.*)
 Lemma body_swapexplicit: semax_body Vprog Gprog f_swap swap_spec.
@@ -232,33 +336,227 @@ Definition swap_writespecx : ident * funspec :=
     PROP () RETURN ()
       SEP (data_at sh1 tint (Vint (Int.repr b)) x; data_at sh2 tint (Vint (Int.repr b)) y).
 
-(*generic swap function template*)
-Definition f_swap (s : statement) := {|
-  fn_return := tvoid;
-  fn_callconv := cc_default;
-  fn_params := ((_x, (tptr tint)) :: (_y, (tptr tint)) :: nil);
-  fn_vars := nil;
-  fn_temps := ((_a2, tint) :: (_b2, tint) :: nil);
-  fn_body :=
-    s
-|}.
 
-(* Packaging the API specs all together. *)
-Definition GprogThree := [swap_spec; swap_readspecx; swap_writespecx].
+      Definition f_swap (s : statement) := {|
+        fn_return := tvoid;
+        fn_callconv := cc_default;
+        fn_params := ((_x, (tptr tint)) :: (_y, (tptr tint)) :: nil);
+        fn_vars := nil;
+        fn_temps := ((_a2, tint) :: (_b2, tint) :: nil);
+        fn_body :=
+          s
+      |}.
+      
+      Definition s := (Ssequence
+      (Sset _a2 (Ederef (Etempvar _x (tptr tint)) tint))
+      (Ssequence
+        (Sset _b2 (Ederef (Etempvar _y (tptr tint)) tint))
+        (Ssequence
+          (Sassign (Ederef (Etempvar _y (tptr tint)) tint) (Etempvar _a2 tint))
+          (Sassign (Ederef (Etempvar _x (tptr tint)) tint) (Etempvar _b2 tint))))).
 
-Definition c : statement := (Ssequence
-(Sset _a2 (Ederef (Etempvar _x (tptr tint)) tint)) Sskip).
+  
+      (*with the exact sequence*)
+  Lemma body_swapsynth: exists s, semax_body Vprog Gprog (f_swap s)  swap_spec.
+  Proof.
+    eexists. 
+    (*partial start function - eliminating fswaps*)
+    leaf_function.
+    lazymatch goal with |- @semax_body ?V ?G ?cs ?F ?spec =>
+    let s := fresh "spec" in
+    pose (s:=spec); hnf in s; cbn zeta in s; (* dependent specs defined with Program Definition often have extra lets *)
+   repeat lazymatch goal with
+    | s := (_, NDmk_funspec _ _ _ _ _) |- _ => fail
+    | s := (_, mk_funspec _ _ _ _ _ _ _) |- _ => fail
+    | s := (_, ?a _ _ _ _) |- _ => unfold a in s
+    | s := (_, ?a _ _ _) |- _ => unfold a in s
+    | s := (_, ?a _ _) |- _ => unfold a in s
+    | s := (_, ?a _) |- _ => unfold a in s
+    | s := (_, ?a) |- _ => unfold a in s
+    end;
+    lazymatch goal with
+    | s :=  (_,  WITH _: globals
+               PRE  [] main_pre _ _ _
+               POST [ tint ] _) |- _ => idtac
+    | s := ?spec' |- _ => check_canonical_funspec spec'
+   end;
+   change (@semax_body V G cs F s); subst s;
+   unfold NDmk_funspec'
+ end;
+ let DependedTypeList := fresh "DependedTypeList" in
+ unfold NDmk_funspec; 
+ match goal with |- semax_body _ _ _ (pair _ (mk_funspec _ _ _ ?Pre _ _ _)) =>
 
-Definition cr : statement := (Ssequence
-(Sset _a2 (Ederef (Etempvar _x (tptr tint)) tint)) Sskip).
-Check Sset.
-Definition cx : statement := 
-(Ssequence
-  (Sset _b2 (Ederef (Etempvar _y (tptr tint)) tint))
-  (Sassign (Ederef (Etempvar _x (tptr tint)) tint) (Etempvar _b2 tint))
-).
-
-
-Lemma body_swapmain: semax_body Vprog GprogThree (f_swap c) swap_spec.
-Proof.
+   split3; [check_parameter_types' | check_return_type | ];
+    match Pre with
+   | (fun _ => convertPre _ _ (fun i => _)) =>  intros Espec DependedTypeList i
+   | (fun _ x => match _ with (a,b) => _ end) => intros Espec DependedTypeList [a b]
+   | (fun _ i => _) => intros Espec DependedTypeList i
+   end;
+   simpl fn_body; simpl fn_params; simpl fn_return
+ end;
+ try match goal with |- semax _ (fun rho => ?A rho * ?B rho) _ _ =>
+     change (fun rho => ?A rho * ?B rho) with (A * B)
+  end;
+ simpl functors.MixVariantFunctor._functor in *;
+ simpl rmaps.dependent_type_functor_rec;
+ clear DependedTypeList;
+ rewrite_old_main_pre;
+ repeat match goal with
+ | |- @semax _ _ _ (match ?p with (a,b) => _ end * _) _ _ =>
+             destruct p as [a b]
+ | |- @semax _ _ _ (close_precondition _ match ?p with (a,b) => _ end * _) _ _ =>
+             destruct p as [a b]
+ | |- @semax _ _ _ ((match ?p with (a,b) => _ end) eq_refl * _) _ _ =>
+             destruct p as [a b]
+ | |- @semax _ _ _ (close_precondition _ ((match ?p with (a,b) => _ end) eq_refl) * _) _ _ =>
+             destruct p as [a b]
+ | |- semax _ (close_precondition _
+                                                (fun ae => !! (Datatypes.length (snd ae) = ?A) && ?B
+                                                      (make_args ?C (snd ae) (mkEnviron (fst ae) _ _))) * _) _ _ =>
+          match B with match ?p with (a,b) => _ end => destruct p as [a b] end
+       end;
+(* this speeds things up, but only in the very rare case where it applies,
+   so maybe not worth it ...
+  repeat match goal with H: reptype _ |- _ => progress hnf in H; simpl in H; idtac "reduced a reptype" end;
+*)
+ try start_func_convert_precondition.
+ Check compute_close_precondition_eq.
+ Check close_precondition_main.
+(*start_function2 does not do anything*)
+ first [ try erewrite compute_close_precondition_eq; [ | reflexivity | reflexivity]
+        | try rewrite close_precondition_main ].
+ (*start function 3.*)
+ simpl app.
+ simplify_func_tycontext.
+ Check mk_funspec.
 Admitted.
+
+Definition lstatement := [Sskip].
+Check lstatement.
+Definition ls2 := lstatement ++ [Sskip].
+Check ls2.
+Print ls2.
+
+
+Definition ssynth := Ssequence
+  (Sset _a2 (Ederef (Etempvar _x (tptr tint)) tint))
+  (Ssequence
+    (Sset _b2 (Ederef (Etempvar _y (tptr tint)) tint))
+    (Ssequence
+      (Sassign (Ederef (Etempvar _y (tptr tint)) tint) (Etempvar _a2 tint))
+      (Sassign (Ederef (Etempvar _x (tptr tint)) tint) (Etempvar _b2 tint)))).
+
+Definition lsequence := [(Sset _a2 (Ederef (Etempvar _x (tptr tint)) tint)); (Sset _b2 (Ederef (Etempvar _y (tptr tint)) tint));
+(Sassign (Ederef (Etempvar _y (tptr tint)) tint) (Etempvar _a2 tint)); (Sassign (Ederef (Etempvar _x (tptr tint)) tint) (Etempvar _b2 tint))].
+Check lsequence.
+
+Fixpoint constructstatement (l : list statement) : statement :=
+  match l with
+  | nil => Sskip
+  | h :: nil => h 
+  | h :: t => (Ssequence h (constructstatement t))
+  end.
+
+Definition stmt := (constructstatement lsequence).
+
+
+(*kinda synthesis*)
+Lemma body_swapsynthesis: semax_body Vprog Gprog (f_swap Sskip)  swap_spec.
+  Proof.
+    start_function.
+    (*go through series of semax Delta P statement P'; till semax Delta P' Sskip POSTC can be proved*)
+    (*first read*)
+    assert(semax Delta 
+    (
+      PROP ( )
+      LOCAL (temp _x x; temp _y y)
+      SEP (data_at sh1 tint (Vint (Int.repr a)) x;
+      data_at sh2 tint (Vint (Int.repr b)) y)
+    )
+    (Sset _a2 (Ederef (Etempvar _x (tptr tint)) tint))
+    (overridePost (
+      PROP ( )
+      LOCAL (temp _a2 (Vint (Int.repr a));temp _x x; temp _y y)
+      SEP (data_at sh1 tint (Vint (Int.repr a)) x;
+      data_at sh2 tint (Vint (Int.repr b)) y)
+    ) POSTCONDITION)). { forward. entailer!. }
+    (*first read stored*)
+    Definition l1 := (Sset _a2 (Ederef (Etempvar _x (tptr tint)) tint)).
+    (*second read*)
+    assert(semax Delta 
+    (
+      PROP ( )
+      LOCAL (temp _a2 (Vint (Int.repr a));temp _x x; temp _y y)
+      SEP (data_at sh1 tint (Vint (Int.repr a)) x;
+      data_at sh2 tint (Vint (Int.repr b)) y)
+    )
+    (Sset _b2 (Ederef (Etempvar _y (tptr tint)) tint))
+    (overridePost (
+      PROP ( )
+      LOCAL (temp _b2 (Vint (Int.repr b));temp _a2 (Vint (Int.repr a));temp _x x; temp _y y)
+      SEP (data_at sh1 tint (Vint (Int.repr a)) x;
+      data_at sh2 tint (Vint (Int.repr b)) y)
+    ) POSTCONDITION)). { forward. entailer!. }
+    Definition list2 := l1 :: [(Sset _b2 (Ederef (Etempvar _y (tptr tint)) tint))].
+    (*first write*)
+    assert(semax Delta 
+    (
+      PROP ( )
+      LOCAL (temp _b2 (Vint (Int.repr b));temp _a2 (Vint (Int.repr a));temp _x x; temp _y y)
+      SEP (data_at sh1 tint (Vint (Int.repr a)) x;
+      data_at sh2 tint (Vint (Int.repr b)) y)
+    )
+    (Sassign (Ederef (Etempvar _y (tptr tint)) tint) (Etempvar _a2 tint))
+    (overridePost (
+      PROP ( )
+      LOCAL (temp _b2 (Vint (Int.repr b));temp _a2 (Vint (Int.repr a));temp _x x; temp _y y)
+      SEP (data_at sh1 tint (Vint (Int.repr a)) x;
+      data_at sh2 tint (Vint (Int.repr a)) y)
+    ) POSTCONDITION)). { forward. entailer!. }
+    (*append list2 to another list: list3*)
+    Definition list3 := list2 ++ [(Sassign (Ederef (Etempvar _y (tptr tint)) tint) (Etempvar _a2 tint))].
+    (*last write x points to b*)
+    assert(semax Delta 
+    (
+      PROP ( )
+      LOCAL (temp _b2 (Vint (Int.repr b));temp _a2 (Vint (Int.repr a));temp _x x; temp _y y)
+      SEP (data_at sh1 tint (Vint (Int.repr a)) x;
+      data_at sh2 tint (Vint (Int.repr a)) y)
+    )
+    (Sassign (Ederef (Etempvar _x (tptr tint)) tint) (Etempvar _b2 tint))
+    (overridePost (
+      PROP ( )
+      LOCAL (temp _b2 (Vint (Int.repr b));temp _a2 (Vint (Int.repr a));temp _x x; temp _y y)
+      SEP (data_at sh1 tint (Vint (Int.repr b)) x;
+      data_at sh2 tint (Vint (Int.repr a)) y)
+    ) POSTCONDITION)). { forward. entailer!. }
+    (*append list3 to another list: list4*)
+    Definition list4 := list3 ++ [(Sassign (Ederef (Etempvar _x (tptr tint)) tint) (Etempvar _b2 tint))].
+    (*Prove Sskip -> POSTC from the established POST in the previous step*)
+    assert(semax Delta 
+    (
+      PROP ( )
+      LOCAL (temp _b2 (Vint (Int.repr b));temp _a2 (Vint (Int.repr a));temp _x x; temp _y y)
+      SEP (data_at sh1 tint (Vint (Int.repr b)) x;
+      data_at sh2 tint (Vint (Int.repr a)) y)
+    )
+    Sskip
+    POSTCONDITION). { unfold POSTCONDITION. unfold abbreviate. forward. entailer!. }
+    (*establsihed; convert list to statement - which is the synthesized program*)
+    Definition synthProg := (constructstatement list4).
+    assert (semax Delta 
+    (
+      PROP ( )
+      LOCAL (temp _x x; temp _y y)
+      SEP (data_at sh1 tint (Vint (Int.repr a)) x;
+      data_at sh2 tint (Vint (Int.repr b)) y)
+    )
+    synthProg
+    POSTCONDITION
+    ). {
+      unfold synthProg. simpl. unfold l1. unfold POSTCONDITION. unfold abbreviate.
+      fastforward.  entailer!.
+    }
+  Admitted.
+
